repair: repair partially the proof
New arguments to AVLNode and a bit of shuffling around.

Signed-off-by: Raito Bezarius <masterancpp@gmail.com>

Verification/BinarySearchTree.lean
@@ -1,9 +1,8 @@
 import Verification.Tree
-import AvlVerification
 
 namespace BST
 
-open Primitives (Result)
+open Primitives (Result Scalar)
 open avl_verification (AVLNode Ordering)
 open Tree (AVLTree AVLNode.left AVLNode.right AVLNode.val)
 
@@ -20,9 +19,10 @@ def AVLNode.mk' (a: T) (left: AVLTree T) (right: AVLTree T): AVLNode T :=
   -- Rust cannot because the height computation will overflow at some point, Rust can only do with trees with representable (usize) height.
   -- It's not big deal because the maximally sized tree is bigger than what modern computer can store at all (exabyte-sized tree).
   AVLNode.mk a left right (@Scalar.ofInt _ height (by sorry))
+
 inductive ForallNode (p: T -> Prop): AVLTree T -> Prop
 | none : ForallNode p none
-| some (a: T) (left: AVLTree T) (right: AVLTree T) : ForallNode p left -> p a -> ForallNode p right -> ForallNode p (some (AVLNode.mk a left right))
+| some (a: T) (left: AVLTree T) (right: AVLTree T) : ForallNode p left -> p a -> ForallNode p right -> ForallNode p (some (AVLNode.mk a left right h))
 
 theorem ForallNode.left {p: T -> Prop} {t: AVLTree T}: ForallNode p t -> ForallNode p t.left := by
   intro Hpt
@@ -36,7 +36,7 @@ theorem ForallNode.right {p: T -> Prop} {t: AVLTree T}: ForallNode p t -> Forall
   | none => simp [AVLTree.right, ForallNode.none]
   | some a left right f_pleft f_pa f_pright => simp [AVLTree.right, f_pright]
 
-theorem ForallNode.label {a: T} {p: T -> Prop} {left right: AVLTree T}: ForallNode p (AVLNode.mk a left right) -> p a := by
+theorem ForallNode.label {a: T} {p: T -> Prop} {left right: AVLTree T}: ForallNode p (AVLNode.mk a left right h) -> p a := by
   intro Hpt
   cases Hpt with 
   | some a left right f_pleft f_pa f_pright => exact f_pa
@@ -73,10 +73,10 @@ inductive Invariant: AVLTree T -> Prop
 | none : Invariant none
 | some (a: T) (left: AVLTree T) (right: AVLTree T) : 
   ForallNode (fun v => v < a) left -> ForallNode (fun v => a < v) right
-  -> Invariant left -> Invariant right -> Invariant (some (AVLNode.mk a left right))
+  -> Invariant left -> Invariant right -> Invariant (some (AVLNode.mk a left right h))
 
 @[simp]
-theorem singleton_bst {a: T}: Invariant (some (AVLNode.mk a none none)) := by
+theorem singleton_bst {a: T}: Invariant (some (AVLNode.mk a none none h)) := by
   apply Invariant.some
   all_goals simp [ForallNode.none, Invariant.none] 
 
@@ -93,7 +93,7 @@ theorem right {t: AVLTree T}: Invariant t -> Invariant t.right := by
   | some _ _ _ _ _ _ _ _ _ => simp [AVLTree.right]; assumption
 
 -- TODO: ask at most for LT + Irreflexive (lt_irrefl) + Trichotomy (le_of_not_lt)?
-theorem left_pos {left right: Option (AVLNode T)} {a x: T}: BST.Invariant (some (AVLNode.mk a left right)) -> x ∈ AVLTree.set (AVLNode.mk a left right) -> x < a -> x ∈ AVLTree.set left := fun Hbst Hmem Hxa => by
+theorem left_pos {left right: Option (AVLNode T)} {a x: T}: BST.Invariant (some (AVLNode.mk a left right h)) -> x ∈ AVLTree.set (AVLNode.mk a left right h) -> x < a -> x ∈ AVLTree.set left := fun Hbst Hmem Hxa => by
    simp [AVLTree.set_some] at Hmem
    rcases Hmem with (Heq | Hleft) | Hright
    . rewrite [Heq] at Hxa; exact absurd Hxa (lt_irrefl _)
@@ -109,7 +109,7 @@ theorem left_pos {left right: Option (AVLNode T)} {a x: T}: BST.Invariant (some 
        exact fun x => le_of_lt
      assumption
  
-theorem right_pos {left right: Option (AVLNode T)} {a x: T}: BST.Invariant (some (AVLNode.mk a left right)) -> x ∈ AVLTree.set (AVLNode.mk a left right) -> a < x -> x ∈ AVLTree.set right := fun Hbst Hmem Hax => by
+theorem right_pos {left right: Option (AVLNode T)} {a x: T}: BST.Invariant (some (AVLNode.mk a left right h)) -> x ∈ AVLTree.set (AVLNode.mk a left right h) -> a < x -> x ∈ AVLTree.set right := fun Hbst Hmem Hax => by
    simp [AVLTree.set_some] at Hmem
    rcases Hmem with (Heq | Hleft) | Hright
    . rewrite [Heq] at Hax; exact absurd Hax (lt_irrefl _)
