Verification/Tree.lean
@@ -1,4 +1,4 @@
-import «AvlVerification»
+import Verification.Extracted
 
 namespace Tree
 
@@ -13,28 +13,35 @@ def AVLTree.nil: AVLTree T := none
 
 def AVLTree.val (t: AVLTree T): Option T := match t with
 | none => none
-| some (AVLNode.mk x _ _) => some x
+| some (AVLNode.mk x _ _ _) => some x
 
 def AVLTree.left (t: AVLTree T): AVLTree T := match t with
 | none => none
-| some (AVLNode.mk _ left _) => left
+| some (AVLNode.mk _ left _ _) => left
 
 def AVLTree.right (t: AVLTree T): AVLTree T := match t with
 | none => none
-| some (AVLNode.mk _ _ right) => right
+| some (AVLNode.mk _ _ right _) => right
+
+def AVLTree.memoized_height (t: AVLTree T): Primitives.Scalar .Usize := match t with
+| none => 0#usize
+| some (AVLNode.mk _ _ _ h) => h
 
 def AVLNode.left (t: AVLNode T): AVLTree T := match t with
-| AVLNode.mk _ left _ => left
+| AVLNode.mk _ left _ _ => left
 
 def AVLNode.right (t: AVLNode T): AVLTree T := match t with
-| AVLNode.mk _ _ right => right
+| AVLNode.mk _ _ right _ => right
 
 def AVLNode.val (t: AVLNode T): T := match t with
-| AVLNode.mk x _ _ => x
+| AVLNode.mk x _ _ _ => x
+
+def AVLNode.memoized_height (t: AVLNode T): Primitives.Scalar .Usize := match t with 
+| AVLNode.mk _ _ _ h => h
 
 mutual
 def AVLTree.height_node (tree: AVLNode T): Nat := match tree with
-| AVLNode.mk y left right => 1 + AVLTree.height left + AVLTree.height right
+| AVLNode.mk y left right _ => 1 + AVLTree.height left + AVLTree.height right
 
 def AVLTree.height (tree: AVLTree T): Nat := match tree with 
 | none => 0
@@ -59,13 +66,13 @@ instance: Coe (Option (AVLNode T)) (AVLTree T) where
 def AVLTree.mem (tree: AVLTree T) (x: T) :=
   match tree with
   | none => False
-  | some (AVLNode.mk y left right) => x = y ∨ AVLTree.mem left x ∨ AVLTree.mem right x
+  | some (AVLNode.mk y left right _) => x = y ∨ AVLTree.mem left x ∨ AVLTree.mem right x
 
 @[simp]
 def AVLTree.mem_none: AVLTree.mem none = ({}: Set T) := rfl
 
 @[simp]
-def AVLTree.mem_some {x: T} {left right: AVLTree T}: AVLTree.mem (some (AVLNode.mk x left right)) = (({x}: Set T) ∪ AVLTree.mem left ∪ AVLTree.mem right) := by
+def AVLTree.mem_some {x: T} {left right: AVLTree T}: AVLTree.mem (some (AVLNode.mk x left right h)) = (({x}: Set T) ∪ AVLTree.mem left ∪ AVLTree.mem right) := by
   ext y
   rw [AVLTree.mem]
   simp [Set.insert_union]
@@ -76,7 +83,7 @@ def AVLTree.mem_some {x: T} {left right: AVLTree T}: AVLTree.mem (some (AVLNode.
 def AVLTree.set (t: AVLTree T): Set T := _root_.setOf (AVLTree.mem t)
 
 @[simp]
-def AVLTree.set_some {x: T} {left right: AVLTree T}: AVLTree.set (some (AVLNode.mk x left right)) = {x} ∪ AVLTree.set left ∪ AVLTree.set right := by 
+def AVLTree.set_some {x: T} {left right: AVLTree T}: AVLTree.set (some (AVLNode.mk x left right h)) = {x} ∪ AVLTree.set left ∪ AVLTree.set right := by 
   simp [set, setOf]
 
 end Tree
